veric/Clight_initial_world.v
@@ -61,13 +61,14 @@ exists fd; split; auto.
 *)
 Qed.
 
-Lemma initial_jm_without_locks m:
+(*Lemma initial_jm_without_locks prog m:
+  Genv.init_mem prog = Some m ->
   (* mem_auth m ∗ *) inflate_initial_mem m ⊢ no_locks.
 Proof.
-  rewrite /no_locks.
-  iIntros "Hm" (?????).
+  rewrite /initial_mem /no_locks.
+  iIntros "(%m & %Hinit & Hm)" (?????).
   iApply (bi.impl_intro_r with "Hm"); iIntros "H".
-Abort.
+Abort.*)
 
 (* How to relate Gamma to funspecs in memory, once we are outside the
    semax proofs?  We define 'matchfunspecs' which will be satisfied by
@@ -80,103 +81,30 @@ Definition matchfunspecs (ge : genv) (G : funspecs) E : mpred :=
    ⌜Genv.find_symbol ge id = Some b /\ find_id id G = Some fs0⌝ ∧
      funspec_sub_si E fs0 fs.
 
-(* How do we prove this? Via initial_core? *)
-
-(*Lemma initial_jm_matchfunspecs prog m G n H H1 H2:
-  matchfunspecs (globalenv prog) G (m_phi (initial_jm prog m G n H H1 H2)).
+Lemma initial_jm_matchfunspecs prog G E:
+  initial_core (globalenv prog) G ⊢ matchfunspecs (globalenv prog) G E.
 Proof.
-  intros b  [fsig cc A P Q ? ?].
-  simpl m_phi.
-  intros phi' ? H0 Hext FAT.
-  simpl in FAT.
-  apply rmap_order in Hext as (Hl & Hr & _).
-  rewrite <- Hr in FAT; clear Hr.
-  assert (H3 := proj2 (necR_PURE' _ _ (b,0) (FUN fsig cc) H0)).
-  spec H3. eauto.
-  destruct H3 as [pp H3].
-  unfold inflate_initial_mem at 1 in H3. rewrite resource_at_make_rmap in H3.
-  unfold inflate_initial_mem' in H3. 
-  destruct (access_at m (b,0) Cur) eqn:Haccess; [ | inv H3].
-  destruct p; try discriminate H3.
-  destruct (initial_core (Genv.globalenv prog) G n @ (b, 0)) eqn:?H; try discriminate H3.
-  inv H3.
-  assert (H3: inflate_initial_mem m (initial_core (Genv.globalenv prog) G n) @ (b,0) = PURE (FUN fsig cc) pp).
-  unfold inflate_initial_mem. rewrite resource_at_make_rmap.
-  unfold inflate_initial_mem'. rewrite H4. rewrite Haccess. auto.
-  unfold initial_core in H4. rewrite resource_at_make_rmap in H4.
-  unfold initial_world.initial_core' in H4. simpl in H4.
-  destruct (Genv.invert_symbol (Genv.globalenv prog) b) eqn:?H; try discriminate.
-  destruct (find_id i G) eqn:?H; try discriminate.
-  destruct f; inv H4.
-  assert (H8 := necR_PURE _ _ _ _ _ H0 H3). clear H0 H3.
-  rewrite FAT in H8.
-  injection H8; intro. subst A0.
-  apply PURE_inj in H8. destruct H8 as [_ H8].
-  simpl in H8.
-  do 2 eexists. split. split. 
-  apply Genv.invert_find_symbol; eauto. eauto.
-  split. split; auto.
-  clear H6 H5 i.
-  rewrite later_unfash.
-  do 3 red.
-  clear FAT. forget (level phi') as n'. rewrite <- Hl in *. clear phi'. clear dependent a''.
-  intros n1' Hn1'. apply laterR_nat in Hn1'.
-  intros ts ftor garg.
-  intros phi Hphi phi' phi'' Hphi' Hext'.
-  apply necR_level in Hphi'. apply ext_level in Hext'.
-  assert (n' > level phi'')%nat by lia.
-  clear n1' Hphi phi Hphi' Hn1' phi' Hext'.
-  rename phi'' into phi.
-  intros [_ ?].
-  assert (approx n' (P ts ftor garg) phi).
-  split; auto.
-  clear H3.
-  apply fupd.fupd_intro.
-  exists ts.
-  assert (H5 := equal_f_dep (equal_f_dep H8 ts) ftor). clear H8.
-  simpl in H5.
-  assert (HP := equal_f (equal_f_dep H5 true) garg).
-  assert (HQ := equal_f_dep H5 false).
-  clear H5.
-   simpl in HP, HQ.
-   rewrite P_ne in H4. rewrite HP in H4. clear HP.
-   change (approx _ (approx _ ?A) _) with ((approx n' oo approx n) A phi) in H4.
-   rewrite fmap_app in H4.
-   rewrite fmap_app in HQ.
-   change (approx _ (approx _ ?A)) with ((approx n' oo approx n) A) in HQ.
-   exists (fmap (dependent_type_functor_rec ts A) (approx n oo approx n')
-             (approx n' oo approx n) ftor).
-  rewrite (approx_min n' n) in *.
-  exists emp. rewrite !emp_sepcon.
-  destruct H4.
-  split. auto.
-  intro rho.
-  pose proof (equal_f HQ rho). simpl in H5.
-  intros phi' Hphi'.
-  rewrite emp_sepcon.
-  intros ? phi'' Hphi'' Hext''.
-  intros [_ ?].
-  rewrite (approx_min n n') in *.
-  rewrite (Nat.min_comm n n') in *.
-  assert (approx (min n' n) (Q0 ts
-       (fmap (dependent_type_functor_rec ts A) (approx (Init.Nat.min n' n))
-          (approx (Init.Nat.min n' n)) ftor) rho) phi'').
-  split; auto.
-  apply necR_level in Hphi''; apply ext_level in Hext''; lia.
-  rewrite <- H5 in H7; clear H5.
-  rewrite <- Q_ne in H7.
-  destruct H7.
-  auto.
-Qed. *)
+  rewrite /initial_core /matchfunspecs.
+  iIntros "#H" (??) "#f".
+  iDestruct ("H" $! b fs) as "[_ Hf]".
+  iDestruct ("Hf" with "f") as %(id & ?%Genv.invert_find_symbol & ?).
+  iExists id, fs; iSplit; first done.
+  iApply funspec_sub_si_refl.
+Qed.
 
 End mpred.
 
+Require Import VST.veric.wsat.
+
+(* Should we compute the block bounds from Genv.init_mem, or leave them arbitrary? *)
 Lemma alloc_initial_state  `{!inG Σ (excl_authR (leibnizO Z))} `{!wsatGpreS Σ} `{!gen_heapGpreS resource' Σ} :
-  forall (prog: program) G n m,
+  forall (prog: program) G z m block_bounds,
       list_norepet (prog_defs_names prog) ->
-      match_fdecs (prog_funct prog) G ->
+      match_fdecs (prog_funct prog) G -> (* this is weird: we need a heapGS to have the funspecs,
+        but we can't have a heap if we haven't allocated the memory yet. *)
       Genv.init_mem prog = Some m ->
-  ⊢ |==> ∃ _ : externalGS Z Σ, ∃ _ : heapGS Σ, ext_auth z ∗ has_ext z ∗ wsat ∗ ownE ⊤ ∗ mem_auth m ∗ inflate_initial_mem m ∗ initial_core m.
+  ⊢ |==> ∃ _ : externalGS Z Σ, ∃ H : heapGS Σ,
+    ext_auth z ∗ has_ext z ∗ wsat ∗ ownE ⊤ ∗ mem_auth m ∗ inflate_initial_mem m block_bounds ∗ initial_world.initial_core(heapGS0 := H) (globalenv prog) G.
 Proof.
   ext_alloc
   alloc_initial_mem
