veric/gen_heap.v
@@ -417,9 +417,11 @@ Proof.
 Qed.
 *)
 
-Lemma gen_heap_init `{!@gen_heapGpreS V Σ ResOps} m σ (Hvalid : ✓ σ)
+Lemma gen_heap_init_names `{!@gen_heapGpreS V Σ ResOps} m σ (Hvalid : ✓ σ)
   (Hcoh : ∀ loc : address, coherent_loc m loc (resource_at σ loc)) :
-  ⊢ |==> ∃ _ : gen_heapGS V Σ, resource_map_auth (gen_heap_name _) Tsh m ∗
+  ⊢ |==> ∃ γh γm,
+    let hG := GenHeapGS V Σ γh γm in
+    resource_map_auth (gen_heap_name _) Tsh m ∗
     ([∗ map] l ↦ x ∈ σ, match x with
                        | shared.YES dq _ v => l ↦{dq} (proj1_sig (elem_of_agree v))
                        | shared.NO sh _ => mapsto_no l sh
@@ -427,7 +429,7 @@ Lemma gen_heap_init `{!@gen_heapGpreS V Σ ResOps} m σ (Hvalid : ✓ σ)
 Proof.
   iMod (resource_map_alloc m σ) as (γh) "(? & ?)".
   iMod (ghost_map_alloc_empty) as (γm) "?".
-  iExists (GenHeapGS _ _ γh γm); iFrame.
+  iExists γh, γm; iFrame.
   rewrite -{1}(big_opM_singletons σ) big_opM_view_frag.
   iPoseProof (big_opM_own_1 with "[-]") as "?"; first done.
   iApply big_sepM_mono; last done; intros ?? Hk.
@@ -445,4 +447,17 @@ Proof.
     split=> b /=; setoid_rewrite elem_of_list_singleton; eauto.
   - rewrite mapsto_no_unseal /mapsto_no_def resource_map.resource_map_elem_no_unseal /resource_map.resource_map_elem_no_def /juicy_view_frag.
     iIntros "?"; iExists rsh; done.
+Qed.
+
+Lemma gen_heap_init `{!@gen_heapGpreS V Σ ResOps} m σ (Hvalid : ✓ σ)
+  (Hcoh : ∀ loc : address, coherent_loc m loc (resource_at σ loc)) :
+  ⊢ |==> ∃ _ : gen_heapGS V Σ, resource_map_auth (gen_heap_name _) Tsh m ∗
+    ([∗ map] l ↦ x ∈ σ, match x with
+                       | shared.YES dq _ v => l ↦{dq} (proj1_sig (elem_of_agree v))
+                       | shared.NO sh _ => mapsto_no l sh
+                       end) ∗ ghost_map_auth (gen_meta_name _) Tsh ∅.
+Proof.
+  iMod (gen_heap_init_names m σ) as (γh γm) "Hinit".
+  iExists (GenHeapGS _ _ γh γm).
+  done.
 Qed.
